c-parser: refactor arch-specific array memory model
This places all arch-specific aspects of the array memory
model in ArchArraysmemInstance.thy.

tools/c-parser/umm_heap/ARM_HYP/ArchArraysMemInstance.thy
@@ -185,25 +185,33 @@ instance num1 :: array_max_count
 (* introduce hackish handling of 8192 type by making a copy of the type
    under a constructor, and then manually showing that it is an instance of
    array_max_count *)
-datatype ty8192 = ty8192 "8192"
+datatype array_max_count_ty = array_max_count_ty "8192"
 
-lemma univ8192: "(UNIV::ty8192 set) = image ty8192 (UNIV::8192 set)"
-apply (simp add: set_eq_iff image_iff)
-apply (rule_tac allI)
-apply (rule_tac ty8192.induct)
-apply simp
-done
+(* ML c-parser code also needs to know at which array size to use this type *)
+ML \<open>
+  structure ArchArrayMaxCount = struct
+    val array_max_count = 8192
+  end
+\<close>
 
-instance "ty8192" :: finite
-apply intro_classes
-apply (simp add: univ8192)
-done
+lemma univ_array_max_count_ty:
+  "(UNIV::array_max_count_ty set) = image array_max_count_ty (UNIV::8192 set)"
+  apply (simp add: set_eq_iff image_iff)
+  apply (rule_tac allI)
+  apply (rule_tac array_max_count_ty.induct)
+  apply simp
+  done
 
-lemma card8192[simp]: "CARD(ty8192) = CARD(8192)"
-apply (simp add: univ8192 card_image inj_on_def)
-done
+instance "array_max_count_ty" :: finite
+  apply intro_classes
+  apply (simp add: univ_array_max_count_ty)
+  done
 
-instance "ty8192" :: array_max_count
+lemma card_array_max_count_ty[simp]: "CARD(array_max_count_ty) = CARD(8192)"
+  apply (simp add: univ_array_max_count_ty card_image inj_on_def)
+  done
+
+instance "array_max_count_ty" :: array_max_count
   by intro_classes simp
 
 end
